I think the tight WCET analysis works for branching and sequential constructs. Now just need to add loops.
Signed-off-by: Avinash Malik <avinash.malik@auckland.ac.nz>

languagedriver.hs
@@ -1,0 +1,96 @@
+module LanguageDrive where
+
+import Language (Cmd(..), Aexp(..), Bexp(..), mkassert, store, computeWcet)
+import qualified Prelude
+import Data.Set as Set
+
+prog1 :: Cmd
+prog1 =
+  Seq (Seq (If (Eq (Avar "init") (Anum ((Prelude.+ 1) 0))) (Assign "m" (Plus
+    (Avar "m") (Anum ((Prelude.+ 1) 0)))) (Assign "u" (Minus (Avar "u") (Anum
+    ((Prelude.+ 1) 0))))) (If (Eq (Avar "Y") (Anum ((Prelude.+ 1) 0)))
+    (Assign "cond" (Bexp0 (Not (Eq (Avar "init") (Anum ((Prelude.+ 1) 0))))))
+    (Assign "cond" (Bexp0 True)))) (If (Eq (Avar "cond") (Bexp0 True))
+    (Assign "m" (Plus (Avar "m") (Anum ((Prelude.+ 1) 0)))) (Assign "u1"
+    (Minus (Avar "u1") (Anum ((Prelude.+ 1) 0)))))
+
+prog2 :: Cmd
+prog2 =
+  Seq (Seq (Assign "X" (Plus (Avar "Y") (Anum ((Prelude.+ 1) ((Prelude.+ 1)
+    ((Prelude.+ 1) ((Prelude.+ 1) ((Prelude.+ 1) ((Prelude.+ 1) 0)))))))))
+    (Assign "X" (Mul (Avar "Y") (Anum ((Prelude.+ 1) ((Prelude.+ 1)
+    ((Prelude.+ 1) ((Prelude.+ 1) ((Prelude.+ 1) ((Prelude.+ 1) 0))))))))))
+    (Assign "X" (Avar "Y"))
+
+
+-- First get all the variables in mkassert
+agetVars :: Aexp -> Set Prelude.String -> Set Prelude.String
+agetVars (Avar x) s = Set.insert x s
+agetVars (Anum _) s = s
+agetVars (Plus l r) s = Set.union (agetVars l s) (agetVars r s)
+agetVars (Minus l r) s = Set.union (agetVars l s) (agetVars r s)
+agetVars (Mul l r) s = Set.union (agetVars l s) (agetVars r s)
+agetVars (Bexp0 b) s = bgetVars b s
+
+bgetVars :: Bexp -> Set Prelude.String -> Set Prelude.String
+bgetVars (Lt l r) s = Set.union (agetVars l s) (agetVars r s)
+bgetVars (Gt l r) s = Set.union (agetVars l s) (agetVars r s)
+bgetVars (Leq l r) s = Set.union (agetVars l s) (agetVars r s)
+bgetVars (Geq l r) s = Set.union (agetVars l s) (agetVars r s)
+bgetVars (Eq l r) s= Set.union (agetVars l s) (agetVars r s)
+bgetVars (And l r) s = Set.union (bgetVars l s) (bgetVars r s)
+bgetVars (Or l r) s = Set.union (bgetVars l s) (bgetVars r s)
+bgetVars (Xor l r) s = Set.union (bgetVars l s) (bgetVars r s)
+bgetVars (Not b) s = bgetVars b s
+bgetVars True s = s
+bgetVars False s = s
+
+-- Now make the smt2-lib string
+amkSMT :: Aexp -> Prelude.String -> Prelude.String
+amkSMT (Avar x) s = s Prelude.++ " " Prelude.++ x
+amkSMT (Anum n) s = s Prelude.++ " " Prelude.++ Prelude.show n
+amkSMT (Plus l r) s = "(+ " Prelude.++ amkSMT l s
+                      Prelude.++ " " Prelude.++ amkSMT r s Prelude.++ ")"
+amkSMT (Minus l r) s = "(- " Prelude.++ amkSMT l s
+                      Prelude.++ " " Prelude.++ amkSMT r s Prelude.++ ")"
+amkSMT (Mul l r) s = "(* " Prelude.++ amkSMT l s
+                      Prelude.++ " " Prelude.++ amkSMT r s Prelude.++ ")"
+amkSMT (Bexp0 b) s = bmkSMT b s
+
+bmkSMT :: Bexp -> Prelude.String -> Prelude.String
+bmkSMT (Lt l r) s = "(< " Prelude.++ amkSMT l s
+                      Prelude.++ " " Prelude.++ amkSMT r s Prelude.++ ")"
+bmkSMT (Gt l r) s = "(> " Prelude.++ amkSMT l s
+                      Prelude.++ " " Prelude.++ amkSMT r s Prelude.++ ")"
+bmkSMT (Leq l r) s = "(<= " Prelude.++ amkSMT l s
+                      Prelude.++ " " Prelude.++ amkSMT r s Prelude.++ ")"
+bmkSMT (Geq l r) s = "(>= " Prelude.++ amkSMT l s
+                      Prelude.++ " " Prelude.++ amkSMT r s Prelude.++ ")"
+bmkSMT (Eq l r) s= "(= " Prelude.++ amkSMT l s
+                      Prelude.++ " " Prelude.++ amkSMT r s Prelude.++ ")"
+bmkSMT (And l r) s = "(and " Prelude.++ bmkSMT l s
+                      Prelude.++ " " Prelude.++ bmkSMT r s Prelude.++ ")"
+bmkSMT (Or l r) s = "(or " Prelude.++ bmkSMT l s
+                      Prelude.++ " " Prelude.++ bmkSMT r s Prelude.++ ")"
+bmkSMT (Xor l r) s = "(xor " Prelude.++ bmkSMT l s
+                      Prelude.++ " " Prelude.++ bmkSMT r s Prelude.++ ")"
+bmkSMT (Not b) s = "(not " Prelude.++ bmkSMT b s Prelude.++ ") "
+bmkSMT True s = "(= 1 1)" Prelude.++ s
+bmkSMT False s = "(= 0 1)" Prelude.++ s
+
+mkSMT :: Cmd -> Prelude.String 
+mkSMT prog = smt where
+  yu = mkassert prog (Eq (Avar "W") (Anum 0))
+       (store (store (store (\_ -> 0) "store" 1) "not" 1) "loop-count" 0)
+  vars = Set.foldr' (\x y -> "(declare-const " Prelude.++ x Prelude.++ " Int) "
+                             Prelude.++ y) "" (bgetVars yu Set.empty)
+  smt' = "\n (assert " Prelude.++ (bmkSMT yu "") Prelude.++ ")"
+  smt = vars Prelude.++ smt'
+
+
+main :: Prelude.IO ()
+main = do
+  Prelude.print (computeWcet
+                 (store (store (store (\_ -> 0) "store" 1) "not" 1)
+                  "loop-count" 0) prog2)
+  Prelude.writeFile  "prog2.smt2" (mkSMT prog2)
