wcet.py
@@ -1,0 +1,33 @@
+#!/usr/bin/env python3
+
+from z3 import Solver, sat, parse_smt2_file, Int
+
+
+def maximise(lb, ub, s, makespan, epsilon=1e-12):
+    if (ub - lb <= epsilon):
+        s.check()
+        return s.model()[makespan]
+    else:
+        half = lb + ((ub - lb)/2.0)
+        s.push()
+        s.add(makespan >= half, makespan <= ub)
+        ret = s.check()
+        s.pop()
+        if ret == sat:
+            return maximise(half, ub, s, makespan, epsilon)
+        else:
+            return maximise(lb, half, s, makespan, epsilon)
+
+
+def main(fname):
+    eqn = parse_smt2_file(fname)
+    W = Int('W')
+    s = Solver()
+    s.add(eqn)
+    print(s)
+    s.check()
+    print('Found WCET for program: %s : %s ' % (fname, s.model()[W]))
+
+
+if __name__ == '__main__':
+    main('prog2.smt2')
